examples/pseudo_bool/graph_encoding/colourScript.sml
@@ -1,7 +1,7 @@
 (*
-  Formalization of the min coloring problem
+  Formalization of the min colouring problem
 *)
-Theory color
+Theory colour
 Ancestors
   pbc graph_basic pbc_normalise mlstring mlint spt_to_vec
 Libs
@@ -9,35 +9,35 @@ Libs
 
 val _ = numLib.temp_prefer_num();
 
-(* f is a k-coloring function on the vertices {0..<v}
-  iff it uses at most k colors ({0..<k}) and
-      no two adjacent vertices have the same color *)
-Definition is_k_color_def:
-  is_k_color k f (v,e) ⇔
+(* f is a k-colouring function on the vertices {0..<v}
+  iff it uses at most k colours ({0..<k}) and
+      no two adjacent vertices have the same colour *)
+Definition is_k_colour_def:
+  is_k_colour k f (v,e) ⇔
   (∀x. x < v ⇒ f x < k) ∧
   (∀x y.
     x < v ∧ y < v ∧ x ≠ y ∧
     is_edge e x y ⇒ f x ≠ f y)
 End
 
-Definition min_color_size_def:
-  min_color_size g =
-  MIN_SET ({k | ∃f. is_k_color k f g})
+Definition min_colour_def:
+  min_colour g =
+  MIN_SET ({k | ∃f. is_k_colour k f g})
 End
 
-Theorem min_color_size_eq:
-  (∀f k'. is_k_color k' f g ⇒ k ≤ k') ∧
-  is_k_color k f g ⇒
-  min_color_size g = k
+Theorem min_colour_eq:
+  (∀f k'. is_k_colour k' f g ⇒ k ≤ k') ∧
+  is_k_colour k f g ⇒
+  min_colour g = k
 Proof
-  rw[min_color_size_def]>>
+  rw[min_colour_def]>>
   DEP_REWRITE_TAC[MIN_SET_TEST_IFF]>>simp[EXTENSION]>>
   metis_tac[]
 QED
 
 (* Color witness:
-  We are given a mapping from {0..<v} to color option
-  And we need to ensure that every vertex is assigned a color
+  We are given a mapping from {0..<v} to colour option
+  And we need to ensure that every vertex is assigned a colour
 *)
 Definition parse_col_header_def:
   (parse_col_header [INL p; _; INR k] =
@@ -103,43 +103,43 @@ Definition parse_col_def:
   parse_col lines = parse_col_toks (MAP toks_num lines)
 End
 
-Definition check_k_color_aux_def:
-  check_k_color_aux k f e v ⇔
+Definition check_k_colour_aux_def:
+  check_k_colour_aux k f e v ⇔
   let c = f v in
   c < k ∧
   let vs = neighbours (e:edges) (v:num) in
   EVERY (λy. y = v ∨ f y ≠ c) vs
 End
 
-Definition check_k_color_def:
-  check_k_color k f (v,e) =
-  EVERY (check_k_color_aux k f e) (COUNT_LIST v)
+Definition check_k_colour_def:
+  check_k_colour k f (v,e) =
+  EVERY (check_k_colour_aux k f e) (COUNT_LIST v)
 End
 
-Theorem check_k_color_is_k_color:
+Theorem check_k_colour_is_k_colour:
   good_graph g ⇒
-  (check_k_color k f g ⇔
-  is_k_color k f g)
+  (check_k_colour k f g ⇔
+  is_k_colour k f g)
 Proof
   `∃v e. g = (v,e)` by metis_tac[PAIR]>>
-  rw[check_k_color_def,is_k_color_def,good_graph_eq,SUBSET_DEF]>>
-  gvs[EVERY_MEM,MEM_COUNT_LIST,check_k_color_aux_def,MEM_neighbours]>>
+  rw[check_k_colour_def,is_k_colour_def,good_graph_eq,SUBSET_DEF]>>
+  gvs[EVERY_MEM,MEM_COUNT_LIST,check_k_colour_aux_def,MEM_neighbours]>>
   eq_tac>>rw[]>>
   gvs[is_edge_def,AllCasePreds()]>>
   metis_tac[]
 QED
 
 Datatype:
-  annot = Edge num num num    (* v1,v2,c: vertices v1, v2 do not both have color c *)
-        | AtLeastOneColor num (* v: vertex v has at-least-one color                *)
-        | AtMostOneColor num  (* v: vertex v has at-most-one color                 *)
-        | VC_Imp_CU num       (* c: vertex-has-color implies color-used            *)
-        | CU_Imp_VC num       (* c: color-used implies vertex-has-color            *)
+  annot = Edge num num num    (* v1,v2,c: vertices v1, v2 do not both have colour c *)
+        | AtLeastOneColor num (* v: vertex v has at-least-one colour                *)
+        | AtMostOneColor num  (* v: vertex v has at-most-one colour                 *)
+        | VC_Imp_CU num       (* c: vertex-has-colour implies colour-used            *)
+        | CU_Imp_VC num       (* c: colour-used implies vertex-has-colour            *)
 End
 
 Datatype:
-  var = VertexHasColor num num (* v,c: vertex v has color c   *)
-      | ColorUsed num          (* c: some vertex uses color c *)
+  var = VertexHasColor num num (* v,c: vertex v has colour c   *)
+      | ColorUsed num          (* c: some vertex uses colour c *)
 End
 
 Definition gen_constraint_def:
@@ -151,12 +151,12 @@ Definition gen_constraint_def:
   (gen_constraint (n:num) ((v,e):graph) (AtLeastOneColor vertex) =
     if vertex < v then
       SOME (GreaterEqual,
-            GENLIST (λcolor. (1i,Pos (VertexHasColor vertex color))) n, 1i)
+            GENLIST (λcolour. (1i,Pos (VertexHasColor vertex colour))) n, 1i)
     else NONE) ∧
   (gen_constraint (n:num) ((v,e):graph) (AtMostOneColor vertex) =
     if vertex < v then
       SOME (GreaterEqual,
-            GENLIST (λcolor. (1i,Neg (VertexHasColor vertex color))) n, & (n - 1))
+            GENLIST (λcolour. (1i,Neg (VertexHasColor vertex colour))) n, & (n - 1))
     else NONE) ∧
   (gen_constraint (n:num) ((v,e):graph) (VC_Imp_CU c) =
     if c < n then
@@ -183,28 +183,28 @@ End
 
 Definition encode_def:
   encode (n:num) ((v,e):graph) =
-    (* every vertex has at least one color *)
+    (* every vertex has at least one colour *)
     flat_genlist v (λvertex.
       gen_named_constraint n (v,e) (AtLeastOneColor vertex)) ++
-    (* every vertex has at most one color *)
+    (* every vertex has at most one colour *)
     flat_genlist v (λvertex.
       gen_named_constraint n (v,e) (AtMostOneColor vertex)) ++
-    (* every color: VC_Imp_CU *)
+    (* every colour: VC_Imp_CU *)
     flat_genlist n (λc.
       gen_named_constraint n (v,e) (VC_Imp_CU c)) ++
-    (* every color: CU_Imp_VC *)
+    (* every colour: CU_Imp_VC *)
     flat_genlist n (λc.
       gen_named_constraint n (v,e) (CU_Imp_VC c)) ++
-    (* for each color: at least one end of each edge does not have that color *)
-    flat_genlist n (λcolor.
+    (* for each colour: at least one end of each edge does not have that colour *)
+    flat_genlist n (λcolour.
       flat_genlist v (λx.
         flat_genlist v (λy.
-          gen_named_constraint n (v,e) (Edge x y color))))
+          gen_named_constraint n (v,e) (Edge x y colour))))
   :(annot # var pbc) list
 End
 
-Definition color_obj_def:
-  color_obj (n:num) =
+Definition colour_obj_def:
+  colour_obj (n:num) =
     SOME (GENLIST (λc. (1, Pos (ColorUsed c))) n,0): ((var lin_term # int) option)
 End
 
@@ -322,15 +322,15 @@ Proof
   \\ rw [] \\ eq_tac \\ rw []
 QED
 
-Definition colors_used_def:
-  colors_used (f:num -> num) v = { c | ∃x. f x = c ∧ x < v }
+Definition colours_used_def:
+  colours_used (f:num -> num) v = { c | ∃x. f x = c ∧ x < v }
 End
 
-Theorem CARD_colors_used_lemma[local]:
+Theorem CARD_colours_used_lemma[local]:
   ∀k n v.
-    is_k_color n f (v,e) ∧ k ≤ n ⇒
-    iSUM (GENLIST (λc. b2i (c ∈ colors_used f v)) k) =
-    & CARD (colors_used f v ∩ count k)
+    is_k_colour n f (v,e) ∧ k ≤ n ⇒
+    iSUM (GENLIST (λc. b2i (c ∈ colours_used f v)) k) =
+    & CARD (colours_used f v ∩ count k)
 Proof
   Induct \\ gvs [iSUM_def,GENLIST,SNOC_APPEND,iSUM_append]
   \\ rw [CARD_INTER_count,GSYM integerTheory.INT_ADD]
@@ -338,26 +338,26 @@ Proof
   \\ first_x_assum $ irule_at Any \\ gvs []
 QED
 
-Theorem CARD_colors_used:
-  is_k_color n f (v,e) ⇒
-  iSUM (GENLIST (λc. b2i (c ∈ colors_used f v)) n) =
-  & CARD (colors_used f v)
+Theorem CARD_colours_used:
+  is_k_colour n f (v,e) ⇒
+  iSUM (GENLIST (λc. b2i (c ∈ colours_used f v)) n) =
+  & CARD (colours_used f v)
 Proof
   rw [] \\ ‘n ≤ n’ by fs []
-  \\ drule_all CARD_colors_used_lemma \\ rw []
+  \\ drule_all CARD_colours_used_lemma \\ rw []
   \\ AP_TERM_TAC
   \\ gvs [EXTENSION]
   \\ rw [] \\ eq_tac \\ rw []
-  \\ gvs [colors_used_def,is_k_color_def]
+  \\ gvs [colours_used_def,is_k_colour_def]
 QED
 
-Theorem is_k_color_IMP_CARD_colors_used_LEQ:
-  is_k_color k f (v,e) ⇒
-  CARD (colors_used f v) ≤ k
+Theorem is_k_colour_IMP_CARD_colours_used_LEQ:
+  is_k_colour k f (v,e) ⇒
+  CARD (colours_used f v) ≤ k
 Proof
   strip_tac
-  \\ qsuff_tac ‘& CARD (colors_used f v) ≤ & k : int’ >- fs []
-  \\ drule CARD_colors_used
+  \\ qsuff_tac ‘& CARD (colours_used f v) ≤ & k : int’ >- fs []
+  \\ drule CARD_colours_used
   \\ disch_then $ rewrite_tac o single o GSYM
   \\ irule iSUM_GENLIST_LEQ
   \\ gvs [EVERY_GENLIST]
@@ -367,26 +367,26 @@ QED
 Theorem encode_correct:
   good_graph (v,e) ⇒
   ((∃f.
-      is_k_color n f (v,e) ∧
-      CARD (colors_used f v) = k)
+      is_k_colour n f (v,e) ∧
+      CARD (colours_used f v) = k)
    ⇔
    (∃w.
       satisfies w (set (MAP SND (encode n (v,e)))) ∧
-      eval_obj (color_obj n) w = & k))
+      eval_obj (colour_obj n) w = & k))
 Proof
   simp [satisfiable_def] \\ rw []
   \\ irule EQ_TRANS
   \\ qexists_tac
-     ‘(∃f. is_k_color n f (v,e) ∧ iSUM (GENLIST (λc. b2i (c ∈ colors_used f v)) n) = & k)’
+     ‘(∃f. is_k_colour n f (v,e) ∧ iSUM (GENLIST (λc. b2i (c ∈ colours_used f v)) n) = & k)’
   \\ conj_tac
   >-
    (AP_TERM_TAC \\ simp [FUN_EQ_THM] \\ rw [] \\ eq_tac \\ rw []
-    \\ imp_res_tac CARD_colors_used \\ gvs [])
+    \\ imp_res_tac CARD_colours_used \\ gvs [])
   \\ eq_tac \\ rw []
   >-
    (qexists_tac ‘λa. case a of
                      | VertexHasColor x c => (f x = c)
-                     | ColorUsed c => c ∈ colors_used f v’
+                     | ColorUsed c => c ∈ colours_used f v’
     \\ gvs [encode_def]
     \\ simp [satisfies_def,MEM_MAP,EXISTS_PROD,flat_genlist_def,
              MEM_FLAT,MEM_GENLIST,PULL_EXISTS,gen_named_constraint_def]
@@ -397,45 +397,45 @@ Proof
       \\ DEP_REWRITE_TAC [iSUM_GE_1]
       \\ conj_tac
       >- simp [EVERY_GENLIST,oneline b2i_def,AllCaseEqs(),EVERY_MAP]
-      \\ gvs [is_k_color_def,MEM_GENLIST,PULL_EXISTS]
+      \\ gvs [is_k_colour_def,MEM_GENLIST,PULL_EXISTS]
       \\ qexists_tac ‘f vertex’ \\ gvs [])
     >-
      (gvs[satisfies_pbc_def,eval_lin_term_def,MAP_GENLIST,o_DEF]
       \\ irule iSUM_one_less
-      \\ gvs [is_k_color_def]
+      \\ gvs [is_k_colour_def]
       \\ last_x_assum drule \\ rw []
       \\ qexists_tac ‘f vertex’ \\ gvs [])
     >-
      (gvs[satisfies_pbc_def,eval_lin_term_def,MAP_GENLIST,o_DEF,iSUM_def]
-      \\ rename [‘c ∈ colors_used f v’]
-      \\ Cases_on ‘c ∈ colors_used f v’ \\ gvs [integerTheory.INT_GE]
+      \\ rename [‘c ∈ colours_used f v’]
+      \\ Cases_on ‘c ∈ colours_used f v’ \\ gvs [integerTheory.INT_GE]
       >-
        (irule ZERO_LE_iSUM
         \\ gvs [EVERY_GENLIST,oneline b2i_def] \\ rw [])
       \\ DEP_REWRITE_TAC [iSUM_EQ_LENGTH]
-      \\ gvs [EVERY_GENLIST,colors_used_def,IN_DEF,oneline b2i_def] \\ rw [])
+      \\ gvs [EVERY_GENLIST,colours_used_def,IN_DEF,oneline b2i_def] \\ rw [])
     >-
      (gvs[satisfies_pbc_def,eval_lin_term_def,MAP_GENLIST,o_DEF,iSUM_def]
-      \\ rename [‘c ∈ colors_used f v’]
-      \\ reverse $ Cases_on ‘c ∈ colors_used f v’ \\ gvs [integerTheory.INT_GE]
+      \\ rename [‘c ∈ colours_used f v’]
+      \\ reverse $ Cases_on ‘c ∈ colours_used f v’ \\ gvs [integerTheory.INT_GE]
       >-
        (DEP_REWRITE_TAC [ZERO_LE_iSUM]
-        \\ gvs [EVERY_GENLIST,colors_used_def,oneline b2i_def,IN_DEF] \\ rw [])
+        \\ gvs [EVERY_GENLIST,colours_used_def,oneline b2i_def,IN_DEF] \\ rw [])
       \\ gvs [GSYM integerTheory.INT_GE]
       \\ DEP_REWRITE_TAC [iSUM_GE_1]
       \\ gvs [MEM_GENLIST,EVERY_GENLIST, oneline b2i_def, AllCaseEqs()]
-      \\ gvs [SF DNF_ss, colors_used_def, IN_DEF]
+      \\ gvs [SF DNF_ss, colours_used_def, IN_DEF]
       \\ first_assum $ irule_at Any \\ gvs [])
     >-
      (Cases_on ‘is_edge e x y ∧ x ≠ y’ \\ gvs []
       \\ simp [satisfies_pbc_def,eval_lin_term_def]
-      \\ gvs [is_k_color_def,MEM_GENLIST,PULL_EXISTS]
+      \\ gvs [is_k_colour_def,MEM_GENLIST,PULL_EXISTS]
       \\ gvs []
       \\ first_x_assum drule_all
-      \\ Cases_on ‘f x = color’ >- gvs [iSUM_def]
-      \\ Cases_on ‘f y = color’ >- gvs [iSUM_def]
+      \\ Cases_on ‘f x = colour’ >- gvs [iSUM_def]
+      \\ Cases_on ‘f y = colour’ >- gvs [iSUM_def]
       \\ gvs [iSUM_def])
-    \\ gvs [color_obj_def,eval_obj_def,eval_lin_term_def,MAP_GENLIST,o_DEF,iSUM_def])
+    \\ gvs [colour_obj_def,eval_obj_def,eval_lin_term_def,MAP_GENLIST,o_DEF,iSUM_def])
   \\ qexists_tac ‘λx. @c. w (VertexHasColor x c) ∧ c < n’
   \\ gvs [encode_def,satisfies_def,MEM_MAP,EXISTS_PROD,flat_genlist_def,
           MEM_FLAT,MEM_GENLIST,PULL_EXISTS,gen_named_constraint_def,SF DNF_ss]
@@ -447,12 +447,12 @@ Proof
     \\ conj_tac
     >- simp [EVERY_GENLIST,oneline b2i_def,AllCaseEqs(),EVERY_MAP]
     \\ gvs [MEM_MAP,PULL_EXISTS,MEM_GENLIST]
-    \\ rw [] \\ qexists_tac ‘color’ \\ gvs []
-    \\ Cases_on ‘w (VertexHasColor x color)’ \\ gvs [])
+    \\ rw [] \\ qexists_tac ‘colour’ \\ gvs []
+    \\ Cases_on ‘w (VertexHasColor x colour)’ \\ gvs [])
   \\ ‘∀x. x < v ⇒ (@c. w (VertexHasColor x c) ∧ c < n) < n ∧
                   w (VertexHasColor x (@c. w (VertexHasColor x c) ∧ c < n))’
     by metis_tac []
-  \\ simp [is_k_color_def]
+  \\ simp [is_k_colour_def]
   \\ rpt strip_tac
   >-
    (rename [‘is_edge e x y’]
@@ -463,16 +463,16 @@ Proof
     \\ simp [] \\ rpt strip_tac \\ gvs []
     \\ first_x_assum $ qspecl_then [‘c_x’,‘x’,‘y’] mp_tac
     \\ simp [satisfies_pbc_def,eval_lin_term_def,iSUM_def])
-  \\ gvs [color_obj_def,eval_obj_def]
+  \\ gvs [colour_obj_def,eval_obj_def]
   \\ rewrite_tac [GSYM integerTheory.INT_OF_NUM_EQ]
-  \\ rewrite_tac [GSYM CARD_colors_used]
+  \\ rewrite_tac [GSYM CARD_colours_used]
   \\ qpat_x_assum ‘_ = &k’ (assume_tac o GSYM)
   \\ asm_rewrite_tac []
   \\ simp [eval_lin_term_def,MAP_GENLIST,o_DEF]
   \\ AP_TERM_TAC
   \\ gvs [listTheory.GENLIST_FUN_EQ] \\ rw []
   \\ AP_TERM_TAC
-  \\ simp [colors_used_def]
+  \\ simp [colours_used_def]
   \\ reverse eq_tac
   >-
    (strip_tac
@@ -491,7 +491,7 @@ Proof
     \\ last_x_assum $ qspec_then ‘u’ kall_tac
     \\ last_x_assum $ qspec_then ‘u’ mp_tac
     \\ gvs [integerTheory.INT_GE,integerTheory.int_le]
-    \\ qabbrev_tac ‘ff = λcolor. 1 − b2i (w (VertexHasColor u color))’
+    \\ qabbrev_tac ‘ff = λcolour. 1 − b2i (w (VertexHasColor u colour))’
     \\ ‘c < d ∨ d < c’ by decide_tac
     >-
      (qspecl_then [‘d’,‘n’,‘ff’] mp_tac GENLIST_SPLIT_LESS \\ simp []
@@ -543,12 +543,12 @@ QED
 Theorem encode_correct_leq:
   good_graph (v,e) ⇒
   ((∃f.
-      is_k_color n f (v,e) ∧
-      CARD (colors_used f v) <= k)
+      is_k_colour n f (v,e) ∧
+      CARD (colours_used f v) <= k)
    ⇔
    (∃w.
       satisfies w (set (MAP SND (encode n (v,e)))) ∧
-      eval_obj (color_obj n) w <= & k))
+      eval_obj (colour_obj n) w <= & k))
 Proof
   strip_tac
   \\ drule encode_correct
@@ -560,13 +560,13 @@ Proof
     \\ strip_tac
     \\ first_x_assum $ irule_at Any
     \\ intLib.COOPER_TAC)
-  \\ ‘0 ≤ eval_obj (color_obj n) w’ by
-   (gvs [color_obj_def,eval_obj_def,eval_lin_term_def,MAP_GENLIST,o_DEF]
+  \\ ‘0 ≤ eval_obj (colour_obj n) w’ by
+   (gvs [colour_obj_def,eval_obj_def,eval_lin_term_def,MAP_GENLIST,o_DEF]
     \\ irule ZERO_LE_iSUM
     \\ gvs [EVERY_GENLIST]
     \\ rw [oneline b2i_def])
   \\ last_x_assum drule
-  \\ disch_then $ qspec_then ‘Num (eval_obj (color_obj n) w)’ mp_tac
+  \\ disch_then $ qspec_then ‘Num (eval_obj (colour_obj n) w)’ mp_tac
   \\ impl_tac >- intLib.COOPER_TAC
   \\ strip_tac
   \\ first_x_assum $ irule_at Any
@@ -575,7 +575,7 @@ QED
 
 Overload toString1 = “λx. toString (x+1n)”
 
-(* NOTE: color is 1-index, vertex is 0-indexed *)
+(* NOTE: colour is 1-index, vertex is 0-indexed *)
 Definition enc_string_def:
   (enc_string (ColorUsed c) = concat [«cu_»; toString1 c]) ∧
   (enc_string (VertexHasColor v c) = concat [«vc_»; toString v; «_»; toString1 c])
@@ -617,7 +617,7 @@ End
 
 Definition full_encode_def:
   full_encode n g =
-  (map_obj enc_string (color_obj n),
+  (map_obj enc_string (colour_obj n),
   MAP (annot_string ## map_pbc enc_string) (encode n g))
 End
 
@@ -716,11 +716,11 @@ QED
 
 (* Check that the objective actually matches up,
   e.g.:
-    map_obj enc_string (color_obj n) = SOME obj
+    map_obj enc_string (colour_obj n) = SOME obj
 *)
-Definition lazy_color_obj_def:
-  lazy_color_obj n (obj: mlstring lin_term # int) ⇔
-    map_obj enc_string (color_obj n) = SOME obj
+Definition lazy_colour_obj_def:
+  lazy_colour_obj n (obj: mlstring lin_term # int) ⇔
+    map_obj enc_string (colour_obj n) = SOME obj
 End
 
 (* Attempt to guess the value of "n" based on the objective.
@@ -747,7 +747,7 @@ Definition lazy_full_encode_def:
   case prob of
     (NONE:mlstring list option,SOME obj, fml) =>
     let n = guess_n obj in
-      if lazy_encode n g fml ∧ lazy_color_obj n obj
+      if lazy_encode n g fml ∧ lazy_colour_obj n obj
       then SOME n
       else NONE
   | _ => NONE
@@ -763,13 +763,13 @@ Proof
   rw[lazy_full_encode_def]>>
   gvs[AllCaseEqs()]>>
   simp[full_encode_def]>>
-  fs[lazy_color_obj_def]>>
+  fs[lazy_colour_obj_def]>>
   drule lazy_encode_imp>>
   simp[MAP_MAP_o]
 QED
 
 (* If the palette allowed is n, then we can claim a lower
-  bound with at most n colors.
+  bound with at most n colours.
   No upper bound is to be used in the PB proof. *)
 Definition conv_concl_def:
   (conv_concl n (OBounds (SOME lb) _) =
@@ -784,7 +784,7 @@ Theorem lazy_full_encode_sem_concl:
   pbc$sem_concl (set (MAP SND fml)) obj {} concl ∧
   conv_concl n concl = SOME lb ⇒
   ∀f k.
-    is_k_color k f g ⇒ lb ≤ k
+    is_k_colour k f g ⇒ lb ≤ k
 Proof
   rw[]>>
   Cases_on`g`>>
@@ -792,8 +792,8 @@ Proof
   simp[PULL_EXISTS, EQ_IMP_THM,SF DNF_ss]>>
   rw[]>>
   pop_assum kall_tac>>
-  ‘~(n < k) ⇒ is_k_color n f (q,r)’ by
-    (gvs [is_k_color_def] >> rw [] >> res_tac >> fs [])>>
+  ‘~(n < k) ⇒ is_k_colour n f (q,r)’ by
+    (gvs [is_k_colour_def] >> rw [] >> res_tac >> fs [])>>
   Cases_on ‘n < k’ >> gvs [] >>
   first_x_assum drule>>rw[]>>
   drule lazy_full_encode_thm >>rw[] >>
@@ -825,7 +825,7 @@ Proof
   ‘∃l. lb = & l’ by (Cases_on ‘lb’ >> gvs []) >>
   gvs [] >>
   rw [] >> irule LESS_EQ_TRANS >> pop_assum $ irule_at Any >>
-  imp_res_tac is_k_color_IMP_CARD_colors_used_LEQ >> fs []
+  imp_res_tac is_k_colour_IMP_CARD_colours_used_LEQ >> fs []
 QED
 
 Theorem full_encode_eq =
@@ -848,7 +848,7 @@ End
 Definition lazy_full_encode_ann_def:
   lazy_full_encode_ann (g:graph) obj anns =
   let n = guess_n obj in
-  if lazy_color_obj n obj
+  if lazy_colour_obj n obj
   then
     OPTION_MAP (\f. (n,f)) (lazy_constraints n g anns [])
   else NONE
@@ -884,7 +884,7 @@ Proof
   rw[lazy_full_encode_ann_def]>>
   gvs[AllCaseEqs()]>>
   simp[full_encode_def]>>
-  fs[lazy_color_obj_def]>>
+  fs[lazy_colour_obj_def]>>
   drule lazy_constraints_subset>>simp[MAP_MAP_o]
 QED
 
@@ -894,7 +894,7 @@ Theorem lazy_full_encode_ann_sem_concl:
   pbc$sem_concl (set fml) (SOME obj) {} concl ∧
   conv_concl n concl = SOME lb ⇒
   ∀f k.
-    is_k_color k f g ⇒ lb ≤ k
+    is_k_colour k f g ⇒ lb ≤ k
 Proof
   rw[]>>
   Cases_on`g`>>
@@ -902,8 +902,8 @@ Proof
   simp[PULL_EXISTS, EQ_IMP_THM,SF DNF_ss]>>
   rw[]>>
   pop_assum kall_tac>>
-  ‘~(n < k) ⇒ is_k_color n f (q,r)’ by
-    (gvs [is_k_color_def] >> rw [] >> res_tac >> fs [])>>
+  ‘~(n < k) ⇒ is_k_colour n f (q,r)’ by
+    (gvs [is_k_colour_def] >> rw [] >> res_tac >> fs [])>>
   Cases_on ‘n < k’ >> gvs [] >>
   first_x_assum drule>>rw[]>>
   drule lazy_full_encode_ann_thm >>rw[] >>
@@ -935,5 +935,5 @@ Proof
   ‘∃l. lb = & l’ by (Cases_on ‘lb’ >> gvs []) >>
   gvs [] >>
   rw [] >> irule LESS_EQ_TRANS >> pop_assum $ irule_at Any >>
-  imp_res_tac is_k_color_IMP_CARD_colors_used_LEQ >> fs []
+  imp_res_tac is_k_colour_IMP_CARD_colours_used_LEQ >> fs []
 QED
