examples/pseudo_bool/array/README.md
@@ -6,8 +6,8 @@ Clique encode and checker
 [cnfProgScript.sml](cnfProgScript.sml):
 CNF encoder and checker
 
-[colorProgScript.sml](colorProgScript.sml):
-Color encode and checker
+[colourProgScript.sml](colourProgScript.sml):
+Colour encode and checker
 
 [compilation](compilation):
 Compiling the pseudo-boolean constraints checker.
