examples/pseudo_bool/array/compilation/README.md
@@ -6,8 +6,8 @@ Compiles the max clique + PB checker
 [cnfCompileScript.sml](cnfCompileScript.sml):
 Compiles the CNF + PB checker
 
-[colorCompileScript.sml](colorCompileScript.sml):
-Compiles the min color + PB checker
+[colourCompileScript.sml](colourCompileScript.sml):
+Compiles the min colour + PB checker
 
 [mccisCompileScript.sml](mccisCompileScript.sml):
 Compiles the MCCIS + PB checker
